SearchAddends implementation

SearchAddends.dfy
@@ -27,6 +27,158 @@ predicate HasAddends(q: seq<int>, x: int)
 	exists i,j :: 0 <= i < j < |q| && q[i] + q[j] == x
 }
 
+predicate IsValidIndex<T>(q: seq<T>, i: nat)
+{
+	0 <= i < |q|
+}
+
+predicate AreOreredIndices<T>(q: seq<T>, i: nat, j: nat)
+{
+	0 <= i < j < |q|
+}
+
+predicate AreAddendsIndices(q: seq<int>, x: int, i: nat, j: nat)
+	requires IsValidIndex(q, i) && IsValidIndex(q, j)
+{
+	q[i] + q[j] == x
+}
+
+predicate HasAddendsInIndicesRange(q: seq<int>, x: int, i: nat, j: nat)
+	requires AreOreredIndices(q, i, j)
+{
+	exists i', j' :: i <= i' < j' <= j < |q| && AreAddendsIndices(q, x, i', j')
+}
+
+predicate LoopInv(q: seq<int>, x: int, i: nat, j: nat, sum: int)
+{
+	AreOreredIndices(q, i, j) && HasAddendsInIndicesRange(q, x, i, j) && AreAddendsIndices(q, sum, i, j)
+}
+
+lemma {:verify true} HasAddendsOnEntry(q: seq<int>, x: int)
+	requires HasAddends(q, x)
+	ensures HasAddendsInIndicesRange(q, x, 0, |q| - 1)
+{
+	calc {
+		HasAddends(q, x);
+		==
+		exists i, j :: 0 <= i < j < |q| && q[i] + q[j] == x;
+		== { assert forall i, j :: (0 <= i < j < |q|) ==> (0 <= i < j <= |q| - 1 < |q|); }
+		exists i, j :: 0 <= i < j <= |q| - 1 < |q| && q[i] + q[j] == x;
+		== {
+			// Extracting this to a lemma doesn't work for some reason
+			assert |q| > 1;
+			assert 0 <= 0 < |q|;
+			assert 0 <= |q| - 1 < |q|;
+			assert forall i, j :: 0 <= i < j <= |q| - 1 < |q| && q[i] + q[j] == x ==> AreAddendsIndices(q, x, i, j);
+		}
+		exists i, j :: 0 <= i < j <= |q| - 1 < |q| && AreAddendsIndices(q, x, i, j);
+		==
+		HasAddendsInIndicesRange(q, x, 0, |q| - 1);
+	}
+}
+
+lemma LoopInvOnEntry(q: seq<int>, x: int, i: nat, j: nat, sum: int)
+	requires sorted: Sorted(q)
+	requires hasAddends: HasAddends(q, x)
+	requires indices: i == 0 && j == |q| - 1
+	requires sum: sum == q[i] + q[j]
+	ensures LoopInv(q, x, i, j, sum)
+{
+	assert |q| > 1 by {
+		reveal hasAddends;
+	}
+	assert AreOreredIndices(q, i, j) by {
+		reveal indices;
+	}
+	assert HasAddendsInIndicesRange(q, x, i, j) by {
+		reveal hasAddends;
+		HasAddendsOnEntry(q, x);
+		reveal indices;
+	}
+	assert AreAddendsIndices(q, sum, i, j) by {
+		reveal sum;
+	}
+}
+
+method FindAddends'(q: seq<int>, x: int) returns (i: nat, j: nat)
+	requires Sorted(q) && HasAddends(q, x)
+	ensures i < j < |q| && q[i] + q[j] == x
+{
+	i := 0;
+	j := |q| - 1;
+	var sum := q[i] + q[j];
+	
+	LoopInvOnEntry(q, x, i, j, sum);
+	while sum != x
+		invariant LoopInv(q, x, i, j, sum)
+		decreases j - i
+	{
+		if (sum > x)
+		{
+			// Sum it too big, lower it by decreasing the high index
+			j := j - 1;
+		}
+		// 'sum == x' cannot occur because the loop's guard is 'sum !=x'.
+		else // (sum < x)
+		{
+			// Sum is too small, make it bigger by increasing the low index.
+			i := i + 1;
+		}
+
+		sum := q[i] + q[j];
+	}
+}
+
 method FindAddends(q: seq<int>, x: int) returns (i: nat, j: nat)
 	requires Sorted(q) && HasAddends(q, x)
 	ensures i < j < |q| && q[i]+q[j] == x
+{
+	i := 0;
+	j := |q| - 1;
+	var sum := q[i] + q[j];
+	
+	LoopInvOnEntry(q, x, i, j, sum);
+	while sum != x
+		invariant LoopInv(q, x, i, j, sum)
+		decreases j - i
+	{
+		assert Sorted(q) && HasAddends(q, x); // from method's pre-condition
+		assert sum != x; // from loop guard;
+		assert LoopInv(q, x, i, j, sum); // from loop invariant
+
+		if (sum > x)
+		{
+			// Sum it too big, lower it by decreasing the high index
+			assert Sorted(q) && HasAddends(q, x); // from method's pre-condition
+			assert sum != x; // from loop guard;
+			assert LoopInv(q, x, i, j, sum); // from loop invariant
+			assert sum > x; // from the if guard
+			// ==>?
+			assert LoopInv(q, x, i, j - 1, q[i] + q[j - 1]);
+			j := j - 1;
+			assert LoopInv(q, x, i, j, q[i] + q[j]);
+		}
+		// 'sum == x' cannot occur because the loop's guard is 'sum !=x'.
+		else // (sum < x)
+		{
+			// Sum is too small, make it bigger by increasing the low index.
+			assert Sorted(q) && HasAddends(q, x); // from method's pre-condition
+			assert sum != x; // from loop guard;
+			assert LoopInv(q, x, i, j, sum); // from loop invariant
+			assert sum < x; // from the negation of the if guard
+			// ==>?
+			assert LoopInv(q, x, i + 1, j, q[i + 1] + q[j]);
+			i := i + 1;
+			assert LoopInv(q, x, i, j, q[i] + q[j]);
+		}
+
+		assert LoopInv(q, x, i, j, q[i] + q[j]);
+		sum := q[i] + q[j];
+		assert LoopInv(q, x, i, j, sum);
+	}
+
+	assert 0 <= i < j < |q| && sum == q[i] + q[j]; // from the loop invariant
+	assert sum == x; // from the negation of the loop guard
+	// ==>
+	assert i < j < |q| && q[i] + q[j] == x;
+}
